updated it_sems_mden4.v (ok)

proofs/itrees/it_sems_mden4.v
@@ -11,37 +11,44 @@ Import Basics.Monads.
 
 From mathcomp Require Import ssreflect ssrfun ssrbool eqtype.
 
-Require Import expr psem_defs psem_core it_exec it_sems_exec tfam_iso1.
+Require Import expr psem_defs psem_core it_exec it_sems_exec tfam_iso1
+               inline_lemmaI2.
 
 Import MonadNotation.
 Local Open Scope monad_scope.
 
+Section Asm1.  
+Context
+  {asm_op: Type} {asmop: asmOp asm_op}.
+(*
+Context
+  {asm_op: Type}
+  {syscall_state : Type}
+  {sip : SemInstrParams asm_op syscall_state}.  
+  {wsw: WithSubWord} 
+  {dc: DirectCall} 
+  {ep : EstateParams syscall_state} 
+  {spp : SemPexprParams} 
+  {pT : progT}
+  {scP : semCallParams}.
+
+Context {err: error_data}. 
+*)
+
 Section Sem1.
 
-Context (FState : Type) {State: Type}.
+Context (FState : Type) {State: Type} {FunDef: Type}.
 
-Notation recCall := (callE (funname * FState) FState).
+(* state events (similar to those provided by the library, 
+   could be specialized to estate) *)
+Variant StE : Type -> Type :=
+  | GetSE : StE State
+  | PutSE : State -> StE unit.                      
 
-Definition rec_call E (f : funname) (fs : FState) :
-   itree (recCall +' E) FState :=
-  trigger_inl1 (Call (f, fs)).
-
-Class sem_Fun (E : Type -> Type) :=
-  { sem_fun : funname -> FState -> itree E FState }.
-
-#[global]
-Instance sem_fun_rec (E : Type -> Type) : sem_Fun (recCall +' E) | 0 :=
-  {| sem_fun := @rec_call E |}.
-(*      fun x y => trigger_inl1 (Call (x, y)) |}. *)
-
-Section Sem2.
-
-Context {Opn: Type}.
-    
-(* state events *)
+(* instruction events *)
 Variant InstrE : Type -> Type :=
   | AssgnE : lval -> assgn_tag -> stype -> pexpr -> InstrE unit
-  | OpnE : lvals -> assgn_tag -> Opn -> pexprs -> InstrE unit
+  | OpnE : lvals -> assgn_tag -> sopn -> pexprs -> InstrE unit
   | SyscallE : lvals -> syscall_t -> pexprs -> InstrE unit
   | EvalCond (e: pexpr) : InstrE bool
   | EvalBound (e: pexpr) : InstrE Z
@@ -50,85 +57,207 @@ Variant InstrE : Type -> Type :=
   | InitFState (args: pexprs) : InstrE FState
   | RetVal (xs: lvals) (fs: FState) (s: State) : InstrE unit.
 
-(* Variant SemFunE : Type -> Type :=
-  | SemFun (fn: funname) (fs: FState) : SemFunE FState.       
-*)  
-
-Variant StE : Type -> Type :=
-  | GetSE : StE State
-  | PutSE : State -> StE unit.                      
-
-End Sem2. 
-
-Section WSW.
-Context
-  {asm_op: Type}
-  {syscall_state : Type}
-  {sip : SemInstrParams asm_op syscall_state}. 
-(*  {wsw: WithSubWord} *)
-(*  {dc: DirectCall} *)
-(*  {ep : EstateParams syscall_state} *)
-(*  {spp : SemPexprParams} *)
-(*  {pT : progT}
-  {scP : semCallParams}. *)
-
-Context {err: error_data}.
-
-Section Sem2a.
-  
-Context {FunDef: Type}.
-
+(* function call events *)
 Variant FunE : Type -> Type :=
   | GetFunDef (fn: funname) (fs: FState) : FunE FunDef
   | GetFunCode (fd: FunDef) : FunE cmd          
   | InitFunCall (fd: FunDef) (fs: FState) : FunE FState                     
   | FinalizeFunCall (fd: FunDef) : FunE FState.
 
-Section Sem3.
-
-Context {E}
-  {XE : ErrEvent -< E} {XI : @InstrE sopn -< E} {XS: StE -< E}.
-(*  {XSF: SemFunE -< E}. *)
-  
-Context (sem_i: instr -> itree E unit).
-
+(* Notation rec_call f fs := (trigger_inl1 (Call (f, fs))). *)
 Local Notation continue_loop := (ret (inl tt)).
 Local Notation exit_loop := (ret (inr tt)).
-  
-(* folding instruction semantics on commands *)
-Definition isem_foldr (c: cmd) : itree E unit :=
+
+(* folding instruction semantics on commands 
+   (without state, it could be simply map) *)
+Definition isem_foldr {E} (sem_i: instr -> itree E unit) (c: cmd) :
+    itree E unit :=
   foldr (fun i k => sem_i i ;; k) (Ret tt) c.
 
-Definition isem_for_round (i : var_i) (c : cmd)
-  (w: Z) (k: itree E unit) : itree E unit :=
-  trigger (WriteIndex i (Vint w)) ;; isem_foldr c ;; k.
+Definition isem_for_round {E} (sem_i: instr -> itree E unit)
+  (wrt: Z -> itree E unit)                        
+  (i : var_i) (c : cmd) (w: Z) (k: itree E unit) : itree E unit :=
+  wrt w ;; isem_foldr sem_i c ;; k.
 
-Definition isem_for_loop (i : var_i) (c : cmd) (ls : list Z)
+Definition isem_for_loop  {E} (sem_i: instr -> itree E unit)
+  (wrt: Z -> itree E unit) 
+  (i : var_i) (c : cmd) (ls : list Z)
   : itree E unit :=
-  foldr (isem_for_round i c) (Ret tt) ls.
+  foldr (isem_for_round sem_i wrt i c) (Ret tt) ls.
 
-Definition isem_while_round (c1 : cmd) (e : pexpr) (c2 : cmd) :
+Definition isem_while_round {E} (sem_i: instr -> itree E unit)
+  (cnd: pexpr -> itree E bool) 
+  (c1 : cmd) (e : pexpr) (c2 : cmd) :
     itree E (unit + unit) :=
-  isem_foldr c1 ;;
-  b <- trigger (EvalCond e) ;;
-  if b then isem_foldr c2 ;; continue_loop 
+  isem_foldr sem_i c1 ;;
+  b <- cnd e ;;
+  if b then isem_foldr sem_i c2 ;; continue_loop 
   else exit_loop.
 
-Definition isem_while_loop (c1 : cmd) (e:pexpr) (c2: cmd) :
+Definition isem_while_loop {E} (sem_i: instr -> itree E unit)
+  (cnd: pexpr -> itree E bool)
+  (c1 : cmd) (e: pexpr) (c2: cmd) :
     itree E unit :=
-  ITree.iter (fun _ => isem_while_round c1 e c2) tt.
+  ITree.iter (fun _ => isem_while_round sem_i cnd c1 e c2) tt.
 
-End Sem3.
+Notation recCall := (callE (funname * FState) FState).
 
-Section Sem3a.
+Section SemRec.
 
-Context {E}
-  {XE : ErrEvent -< E} {XI : @InstrE sopn -< E} {XS: StE -< E}
-  {sem_F : sem_Fun E }.
-(*  {XR: recCall -< E}. *)
-(*  {XR: FIso E (recCall +' E0)}. *)
+Context {E} {XI : InstrE -< E} {XS: StE -< E}.
 
-(* Context (sem_i: instr -> itree E unit). *)
+(* semantics of instructions *)
+Fixpoint isem_instr (i : instr) : itree (recCall +' E) unit :=
+  let: (MkI _ ir) := i in
+  match ir with
+  | Cassgn x tg ty e => trigger (AssgnE x tg ty e)
+
+  | Copn xs tg o es => trigger (OpnE xs tg o es)
+
+  | Csyscall xs o es => trigger (SyscallE xs o es) 
+                                
+  | Cif e c1 c2 =>
+    b <- trigger (EvalCond e) ;;
+    isem_foldr isem_instr (if b then c1 else c2) 
+               
+  | Cwhile a c1 e i c2 =>
+      isem_while_loop isem_instr (fun e => trigger (EvalCond e))
+        c1 e c2 
+
+  | Cfor i (d, lo, hi) c =>
+    lo_b <- trigger (EvalBound lo) ;;
+    hi_b <- trigger (EvalBound hi) ;;   
+    isem_for_loop isem_instr (fun w => trigger (WriteIndex i (Vint w)))
+      i c (wrange d lo_b hi_b) 
+
+  | Ccall xs fn args =>
+    s0 <- trigger GetSE ;;  
+    vargs <- trigger (EvalArgs args) ;;
+    fs0 <- trigger (InitFState vargs) ;;
+    fs1 <- trigger_inl1 (Call (fn, fs0)) ;; 
+    (* discard current state, use s0 instead *)
+    trigger (RetVal xs fs1 s0)
+(* | _ => throw err end. *)
+  end.
+
+(* semantics of commands *)
+Definition isem_cmd c := isem_foldr isem_instr c.
+
+Section SemFun.
+
+Context {XF: FunE -< E}.  
+
+(* semantics of function calls *)
+Definition isem_fcall (fn : funname) (fs : FState) :
+  itree (recCall +' E) FState :=
+  fd <- trigger (GetFunDef fn fs) ;;  
+  c <- trigger (GetFunCode fd) ;;
+  trigger (InitFunCall fd fs) ;;
+  isem_cmd c ;;
+  trigger (FinalizeFunCall fd).
+
+(************************************************************)
+(* full function semantics *)
+
+(* handler of recCall events *)
+Definition handle_recc : recCall ~> itree (recCall +' E) :=
+ fun T (rc : recCall T) =>
+   match rc with
+   | Call (fn, fs) => isem_fcall fn fs
+   end.
+
+(* intepreter of recCall events *)
+Definition interp_recc T (t: itree (recCall +' E) T) : itree E T :=
+  interp_mrec handle_recc t.
+
+(* recCall interpreter of instructions *)
+Definition denote_instr (i: instr) : itree E unit :=
+  interp_recc (isem_instr i).
+
+(* recCall interpreter of commands *)
+Definition denote_cmd (c: cmd) : itree E unit :=
+  interp_recc (isem_cmd c).
+
+(* recCall interpreter of function calls *)
+Definition denote_fun (fn : funname) (fs : FState) : itree E FState :=
+  interp_recc (isem_fcall fn fs).
+
+(* function semantics, directly expressed with rec *)
+Definition denote_fcall (fn : funname) (fs : FState) : itree E FState :=
+  rec (uncurry isem_fcall) (fn, fs). 
+
+(********************************************************************)
+(* blank function semantics *)
+
+Definition rec_call (f : funname) (fs : FState) :
+   itree (recCall +' E) FState := trigger_inl1 (Call (f, fs)).
+
+(* fully blank semantics (does nothing) *)
+Definition denote_fcall_blank (fn : funname) (fs : FState) : itree E FState :=
+  rec (uncurry rec_call) (fn, fs). 
+
+(* blank handler of recCall events *)
+Definition handle_recc_blank : recCall ~> itree (recCall +' E) :=
+ fun T (rc : recCall T) =>
+   match rc with
+   | Call (fn, fs) => trigger_inl1 (Call (fn, fs))
+   end.
+
+(* uninterpreted function semantics *)
+Definition denote_fun_blank (fn : funname) (fs : FState) : itree E FState :=
+  interp_mrec handle_recc_blank (isem_fcall fn fs).
+
+(**********************************************************************)
+
+Lemma denote_cmd_cons_eutt i c :
+  eutt eq (denote_cmd (i :: c))
+          (denote_instr i ;; denote_cmd c).       
+Proof.
+  setoid_rewrite interp_mrec_as_interp; simpl.
+  setoid_rewrite interp_bind; reflexivity.
+Qed.
+
+Lemma denote_fun_eutt (fn : funname) (fs : FState) :
+  eutt eq (denote_fcall fn fs) (denote_fun fn fs).
+Proof. by reflexivity. Qed.  
+
+Lemma denote_fun_blank_eutt (fn : funname) (fs : FState) :
+  eutt eq (denote_fcall_blank fn fs) (denote_fun_blank fn fs).
+Proof.
+  unfold denote_fcall_blank, denote_fun_blank, rec, mrec.
+  setoid_rewrite interp_mrec_as_interp.
+  eapply eutt_interp; eauto; try reflexivity.
+  simpl. unfold isem_fcall.
+  unfold rec_call.
+Abort.
+
+Lemma denote_fun_blank_eutt (fn : funname) (fs : FState) :
+  eutt eq (denote_fun fn fs) (denote_fun_blank fn fs).
+Proof.
+  unfold denote_fun, denote_fun_blank, rec, mrec.
+  setoid_rewrite interp_mrec_as_interp.
+  eapply eutt_interp; eauto; try reflexivity.
+  unfold eq2, Eq2_Handler, eutt_Handler, Relation.i_pointwise.
+  intros.
+Abort.
+  
+End SemFun.
+
+End SemRec.
+
+
+Class sem_Fun (E : Type -> Type) :=
+  { sem_fun : funname -> FState -> itree E FState }.
+
+#[global]
+Instance sem_fun_rec (E : Type -> Type) : sem_Fun (recCall +' E) | 0 :=
+  {| sem_fun := @rec_call E |}.
+  
+Section SemPRec.
+
+Context {E} {XI : InstrE -< E} {XS: StE -< E} {sem_F : sem_Fun E }.
+  
+Context (sem_i: instr -> itree E unit).
 
 (* semantics of instructions, abstracting on function calls (through
    sem_fun) *)
@@ -146,12 +275,14 @@ Fixpoint isem_i_body (i : instr) : itree E unit :=
     isem_foldr isem_i_body (if b then c1 else c2) 
                
   | Cwhile a c1 e i c2 =>
-    isem_while_loop isem_i_body c1 e c2 
+      isem_while_loop isem_i_body (fun e => trigger (EvalCond e))
+        c1 e c2 
 
   | Cfor i (d, lo, hi) c =>
     lo_b <- trigger (EvalBound lo) ;;
     hi_b <- trigger (EvalBound hi) ;;   
-    isem_for_loop isem_i_body i c (wrange d lo_b hi_b) 
+    isem_for_loop isem_i_body (fun w => trigger (WriteIndex i (Vint w)))
+      i c (wrange d lo_b hi_b) 
 
   | Ccall xs fn args =>
     s0 <- trigger GetSE ;;  
@@ -162,74 +293,50 @@ Fixpoint isem_i_body (i : instr) : itree E unit :=
     trigger (RetVal xs fs1 s0)
 (* | _ => throw err end. *)
   end.
+
 (* similar, for commands *)
-Definition isem_cmd_ c := isem_foldr isem_i_body c.
+Definition isem_c_body c := isem_foldr isem_i_body c.
 
-End Sem3a.
+Section SemPFun.
 
-(* Definition estate0 (fs : fstate) :=
-  Estate fs.(fscs) fs.(fmem) Vm.init. *)
-
-Section Sem4.
-
-Context {E}
-  {XE : ErrEvent -< E} {XI : @InstrE sopn -< E} {XS: StE -< E}
-  {XR: recCall -< E} {sem_F : sem_Fun E }.
-
-Context {XF: FunE -< E}.
-
-(* Context (sem_i: instr -> itree E unit). *)
+Context {XF: FunE -< E}.  
 
 Definition isem_fun_body (fn : funname) (fs : FState) : itree E FState :=
   fd <- trigger (GetFunDef fn fs) ;;  
   c <- trigger (GetFunCode fd) ;;
   trigger (InitFunCall fd fs) ;;
-  isem_cmd_ (E := E) c ;; 
+  isem_c_body c ;; 
   trigger (FinalizeFunCall fd).
 
-End Sem4.
+End SemPFun.
 
-Section Sem3b.
+End SemPRec.
 
+Section SemA.
+  
 Context {E}
-  {XE : ErrEvent -< E} {XI : @InstrE sopn -< E} {XS: StE -< E}.
+  {XE : ErrEvent -< E} {XI : InstrE -< E} {XS: StE -< E}.
 
 Context {XF: FunE -< E}.
 
 Context (sem_i: instr -> itree (recCall +' E) unit).
 
+(************************************************************)
+(* uninterpreted function semantics *)
+
 (* semantics of instructions parametrized by recCall events *)
-Definition isem_i_rec (i : instr) 
-  : itree (recCall +' E) unit :=
-  @isem_i_body (recCall +' E) (fun T e => inr1 (@XI T e))
-    (fun T e => inr1 (@XS T e)) (sem_fun_rec E) i.
-
-(* similar, for commands *)
-Definition isem_cmd_rec (c : cmd)
-  : itree (recCall +' E) unit :=
-  @isem_cmd_ (recCall +' E) (fun T e => inr1 (@XI T e))
-     (fun T e => inr1 (@XS T e)) (sem_fun_rec E) c.
-
-(* similar, for function calls *)
-Definition isem_fun_rec 
-   (fn : funname) (fs : FState) : itree (recCall +' E) FState :=
-  @isem_fun_body (recCall +' E) (fun T e => inr1 (@XI T e))
-    (fun T e => inr1 (@XS T e)) (sem_fun_rec E)
-    (fun T e => inr1 (@XF T e)) fn fs.
-
-(*
-Definition handle_trivial_SemFun T (e: SemFunE T) : itree (recCall +' E) T :=
-  match e with
-  | SemFun fn fs => trigger (inl1 (Call (fn, fs))) end.
-
-Definition handle_trivial_SemFun' T (e: E T) : itree (recCall +' E) T :=
-  match mfun1 e with
-  | inl1 e1 => @handle_trivial_SemFun T e1
-  | _ => trigger (inr1 e) end.                                               
+Definition isem_i_rec (i : instr) : itree (recCall +' E) unit :=
+  isem_i_body i.
   
-Definition interp_SemFun T (t: itree E T) : itree (recCall +' E) T :=
-  interp handle_trivial_SemFun' t.
-*)
+Definition isem_cmd_rec (c : cmd) : itree (recCall +' E) unit :=
+  isem_c_body c.
+
+Definition isem_fun_rec 
+  (fn : funname) (fs : FState) : itree (recCall +' E) FState :=
+  isem_fun_body fn fs.
+
+(************************************************************)
+(* full function semantics *)
 
 (* handler of recCall events *)
 Definition handle_recCall :
@@ -238,6 +345,10 @@ Definition handle_recCall :
    match rc with
    | Call (fn, fs) => isem_fun_rec fn fs
    end.
+
+(* intepreter of recCall events *)
+Definition interp_recCall T (t: itree (recCall +' E) T) : itree E T :=
+  interp_mrec handle_recCall t.
 
 (* intepreter of recCall events for functions, giving us the recursive
    semantics of functions *)
@@ -250,660 +361,54 @@ Instance sem_fun_full : sem_Fun E | 100 :=
 
 (* recursive semantics of instructions *)
 Definition isem_i (i : instr) : itree E unit :=
-  @isem_i_body E XI XS sem_fun_full i.
+  isem_i_body i.
 
 (* similar, for commands *)
-Definition isem_cmd (c : cmd) : itree E unit :=
-  isem_cmd_ c.
+Definition isem_c (c : cmd) : itree E unit :=
+  isem_c_body c.
 
 (************************************************************)
+(* blank function semantics *)
 
-
-Definition isem_i_rec (i : instr) 
-  : itree (recCall +' E) unit :=
-  @isem_i_body (recCall +' E)
-    (fun T e => inr1 (XI e))
-    (fun T e => inr1 (XS e)) inl1 sem_i i.
-
-Definition isem_cmd_rec (c : cmd) 
-  : itree (recCall +' E) unit :=
-  isem_cmd_ sem_i c.
-
-Definition isem_fun_rec 
-   (fn : funname) (fs : FState) : itree (recCall +' E) FState :=
-  @isem_fun_body (recCall +' E) 
-    (fun T e => inr1 (XF e)) sem_i fn fs.
-
-(* handler of recCall events *)
-Definition handle_recCall :
+(* blank recCall handler *)
+Definition handle_recCallB :
    recCall ~> itree (recCall +' E) :=
  fun T (rc : recCall T) =>
    match rc with
-   | Call (fn, fs) => isem_fun_rec fn fs
+   | Call (fn, fs) => rec_call fn fs
    end.
 
-(* intepreter of recCall events for functions, giving us the recursive
-   semantics of functions *)
-(* Definition isem_fun (fn : funname) (fs : FState) : itree E FState :=
-  mrec handle_recCall (Call (fn, fs)). *)
-Definition interp_recCall T (t: itree (recCall +' E) T) : itree E T :=
-  interp_mrec handle_recCall t.
+(* blank recCall interpreter (non-terminating) *)
+Definition interp_recCallB T (t: itree (recCall +' E) T) : itree E T :=
+  interp_mrec handle_recCallB t.
 
-(***)
+(* blank function semantics *)
+Definition isem_funB (fn : funname) (fs : FState) : itree E FState :=
+  mrec handle_recCallB (Call (fn, fs)).
 
-Definition isem_fun (fn : funname) (fs : FState) : itree E FState :=
-  mrec handle_recCall (Call (fn, fs)). 
+(*********************************************************************)
 
+Lemma isem_fun_rec_eutt (fn : funname) (fs : FState) :
+  eutt eq (isem_fun_rec fn fs) (isem_fcall fn fs).
+Proof. by reflexivity. Qed.
 
-(*
-Definition handle_trivial_SemFun T (e: SemFunE T) : itree (recCall +' E) T :=
-  match e with
-  | SemFun fn fs => trigger (inl1 (Call (fn, fs))) end.
+Lemma interp_recCall_eutt T (t: itree (recCall +' E) T) :
+  eutt eq (interp_recCall t) (interp_recc t).
+Proof.
+  unfold interp_recCall, interp_recc.
+  eapply interp_mrec_eqit with (VRel := @eq); try reflexivity.
+  intros V k1 k2 H v1 v2 H0.
+  inv H0; eauto.
+Qed.
 
-Definition handle_trivial_SemFun' T (e: E T) : itree (recCall +' E) T :=
-  match mfun1 e with
-  | inl1 e1 => @handle_trivial_SemFun T e1
-  | _ => trigger (inr1 e) end.                                               
+End SemA.
   
-Definition interp_SemFun T (t: itree E T) : itree (recCall +' E) T :=
-  interp handle_trivial_SemFun' t.
-*)
+End Sem1.
 
-(*
-Definition initialize_funcall (fd : fundef) (fs : fstate) : exec estate :=
-  let sinit := estate0 fs in
-  Let vargs' := mapM2 ErrType dc_truncate_val fd.(f_tyin) fs.(fvals) in
-  Let s0 := init_state fd.(f_extra) (p_extra p) ev sinit in
-  write_vars (~~direct_call) fd.(f_params) vargs' s0.
+End Asm1.
 
-Definition finalize_funcall (fd : fundef) (s:estate) : exec fstate :=
-  Let vres := get_var_is (~~ direct_call) s.(evm) fd.(f_res) in
-  Let vres' := mapM2 ErrType dc_truncate_val fd.(f_tyout) vres in
-  let scs := s.(escs) in
-  let m := finalize fd.(f_extra) s.(emem) in
-  ok {| fscs := scs; fmem := m; fvals := vres' |}.
 
-Definition ifinalize_funcall (fd : fundef) (s:estate) : itree E fstate :=
-  err_result (fun e => (e, tt)) (finalize_funcall fd s).
 
-(* similar, for proper function calls *)
-Definition isem_fun_body (p : prog) (ev : extra_val_t)
-   (fn : funname) (fs : fstate) :=
-   fd <- kget_fundef (p_funcs p) fn fs;;
-   let sinit := estate0 fs in
-   s1 <- iresult sinit (initialize_funcall p ev fd fs);;
-   s2 <- isem_cmd_ p ev fd.(f_body) s1;;
-   iresult s2 (finalize_funcall fd s2).
-*)
 
-(*
-(**** Error semantics ******************************************)
-Section Errors.
 
-(* error events *)
-Definition ErrEvent : Type -> Type := exceptE error_data.
 
-(* execT (itree E) R = itree E (execS R) *)
-Definition handle_Err {E} : ErrEvent ~> execT (itree E) :=
-  fun _ e =>
-    match e with
-    | Throw e' => Ret (ESerror _ e')
-    end.
-
-(* ErrEvnt handler *)
-Definition ext_handle_Err {E: Type -> Type} :
-  ErrEvent +' E ~> execT (itree E) :=
-  fun _ e =>
-  match e with
-  | inl1 e' => handle_Err e'
-  | inr1 e' => Vis e' (pure (fun x => ESok x)) end.
-
-(* ErrEvent interpreter *)
-Definition interp_Err {E: Type -> Type} {A}
-  (t: itree (ErrEvent +' E) A) : execT (itree E) A :=
-  interp_exec ext_handle_Err t.
-
-(*** auxiliary error functions *)
-
-Definition ioget {E: Type -> Type} `{ErrEvent -< E} {V} (err: error_data) (o: option V) : itree E V :=
-  match o with
-  | Some v => Ret v
-  | None => throw err
-  end.
-
-Definition err_result {E: Type -> Type} `{ErrEvent -< E} (Err : error -> error_data) :
-  result error ~> itree E :=
-  fun _ t => match t with
-             | Ok v => Ret v
-             | Error e => throw (Err e) end.
-
-End Errors.
-
-(** Type function isomorphism class *)
-Class FIso (E1 E2: Type -> Type) : Type := FI {
-    mfun1 : E1 -< E2 ;
-    mfun2 : E2 -< E1 ;
-    mid12 : forall T (x : E2 T), mfun1 (mfun2 x) = x ;
-    mid21 : forall T (x : E1 T), mfun2 (mfun1 x) = x ;
-}.
-
-Notation with_Error E E0 := (FIso E (ErrEvent +' E0)).
-
-#[global] Instance fromErr E E0 {wE : with_Error E E0} : ErrEvent -< E :=
-  fun T (e:ErrEvent T) => mfun2 (inl1 e).
-
-Definition is_error {E E0 : Type -> Type} (wE : with_Error E E0) (T : Type) (e : E T) :=
-  match mfun1 e with
-  | inl1 _ => true
-  | inr1 _ => false
-  end.
-
-(* with_Error (ErrEvent +' void1) void1 *)
-#[global]
-Instance FIsoId E : FIso E E :=
-  {| mfun1 := fun T x => x
-   ; mfun2 := fun T x => x
-   ; mid12 := fun T x => erefl
-   ; mid21 := fun T x => erefl |}.
-
-(* with_Error E E0 -> with_Error (E1 +' E) (E1 +' E0) *)
-Section FIso_suml.
-Context (E1 E E0 Err : Type -> Type) {FI : FIso E (Err +' E0)}.
-
-Definition mfun1_suml T (e : (E1 +' E) T) : (Err +' (E1 +' E0)) T :=
-  match e with
-  | inl1 e1 => inr1 (inl1 e1)
-  | inr1 e =>
-    match mfun1 e with
-    | inl1 err => inl1 err
-    | inr1 e0  => inr1 (inr1 e0)
-    end
-  end.
-
-Definition mfun2_suml T (e : (Err +' (E1 +' E0)) T) : (E1 +' E) T :=
-  match e with
-  | inl1 err => inr1 (mfun2 (inl1 err))
-  | inr1 e10 =>
-    match e10 with
-    | inl1 e1 => inl1 e1
-    | inr1 e0  => inr1 (mfun2 (inr1 e0))
-    end
-  end.
-
-Lemma mfun_suml_12 T (x : (Err +' (E1 +' E0)) T) :
-  mfun1_suml (mfun2_suml x) = x.
-Proof. by case: x => [err | [e1 | e0]] //=; rewrite ?(mid12, mid21). Qed.
-
-Lemma mfun_suml_21 T (x : (E1 +' E) T) :
-  mfun2_suml (mfun1_suml x) = x.
-Proof.
-  case: x => [e1 | e] //=.
-  by case heq : (mfun1 e) => [err | e0] /=; rewrite -heq ?(mid12, mid21).
-Qed.
-
-#[global]
-Instance FIso_suml : FIso (E1 +' E) (Err +' (E1 +' E0)) :=
-  {| mfun1 := mfun1_suml
-   ; mfun2 := mfun2_suml
-   ; mid12 := mfun_suml_12
-   ; mid21 := mfun_suml_21 |}.
-
-End FIso_suml.
-
-*)
-
-Section WSW.
-Context
-  {asm_op: Type}
-  {wsw: WithSubWord}
-  {dc: DirectCall}
-  {syscall_state : Type}
-  {ep : EstateParams syscall_state}
-  {spp : SemPexprParams}
-  {sip : SemInstrParams asm_op syscall_state}
-  {pT : progT}
-  {scP : semCallParams}.
-
-Record fstate := { fscs : syscall_state_t; fmem : mem; fvals : values }.
-
-(* Recursion events (curried version of Call in ITree) *)
-Variant recCall : Type -> Type :=
- | RecCall (f:funname) (fs:fstate) : recCall fstate.
-
-Definition mk_error_data (s:estate) (e:error)  := (e, tt).
-
-Definition mk_errtype := fun s => mk_error_data s ErrType.
-
-(**** Auxiliary definitions ******************************************)
-Section CORE.
-
-Context {E E0} {wE : with_Error E E0} (p : prog) (ev : extra_val_t).
-
-Definition kget_fundef (funcs: fun_decls) (fn: funname) :
-    ktree E fstate fundef :=
-  fun _ => ioget (ErrType, tt) (get_fundef funcs fn).
-
-Definition iresult {T} (s:estate) (F : exec T)  : itree E T :=
-  err_result (mk_error_data s) F.
-
-Definition iwrite_var (wdb : bool) (x : var_i) (v : value) (s : estate) :
-    itree E estate :=
-  iresult s (write_var wdb x v s).
-
-Definition iwrite_lval (wdb : bool) (gd : glob_decls) (x : lval)
-    (v : value) (s : estate) : itree E estate :=
-  iresult s (write_lval wdb gd x v s).
-
-Definition iwrite_lvals (wdb : bool) (gd : glob_decls) (xs : lvals)
-    (vs : values) (s : estate) : itree E estate :=
-  iresult s (write_lvals wdb gd s xs vs).
-
-Definition isem_pexprs (wdb : bool) (gd : glob_decls) (es: pexprs)
-    (s : estate) : itree E values :=
-  iresult s (sem_pexprs wdb gd s es).
-
-Definition sem_assgn  (x : lval) (tg : assgn_tag) (ty : stype) (e : pexpr)
-    (s : estate) : exec estate :=
-  Let v := sem_pexpr true (p_globs p) s e in
-  Let v' := truncate_val ty v in
-  write_lval true (p_globs p) x v' s.
-
-Definition fexec_syscall (o : syscall_t) (fs:fstate) : exec fstate :=
-  Let: (scs, m, vs) := exec_syscall fs.(fscs) fs.(fmem) o fs.(fvals) in
-  ok {| fscs := scs; fmem := m; fvals := vs |}.
-
-Definition mk_fstate (vs:values) (s:estate) :=
-  {| fscs := escs s; fmem:= emem s; fvals := vs |}.
-
-Definition upd_estate wdb (gd : glob_decls) (xs:lvals) (fs : fstate)
-    (s:estate) :=
-  write_lvals wdb gd (with_scs (with_mem s fs.(fmem)) fs.(fscs)) xs fs.(fvals).
-
-Definition sem_syscall (xs : lvals) (o : syscall_t) (es : pexprs)
-    (s : estate) : exec estate :=
-  Let ves := sem_pexprs true (p_globs p) s es in
-  Let fs := fexec_syscall o (mk_fstate ves s) in
-  upd_estate true (p_globs p) xs fs s.
-
-Definition sem_cond (gd : glob_decls) (e : pexpr) (s : estate) : exec bool :=
-  (sem_pexpr true gd s e >>= to_bool)%result.
-
-Definition isem_cond (e : pexpr) (s : estate) : itree E bool :=
-  iresult s (sem_cond (p_globs p) e s).
-
-Definition sem_bound (gd : glob_decls) (lo hi : pexpr) (s : estate) :
-    exec (Z * Z) :=
-  (Let vlo := sem_pexpr true gd s lo >>= to_int in
-  Let vhi := sem_pexpr true gd s hi >>= to_int in
-  ok (vlo, vhi))%result.
-
-Definition isem_bound (lo hi : pexpr) (s : estate) : itree E (Z * Z) :=
-  iresult s (sem_bound (p_globs p) lo hi s).
-
-(* recCall trigger *)
-Definition rec_call (f : funname) (fs : fstate) :
-   itree (recCall +' E) fstate :=
-  trigger_inl1 (RecCall f fs).
-
-End CORE.
-
-(**** Abstract semantics **********************************************)
-Section SEM_C.
-
-Context {E E0} {wE : with_Error E E0}
-        (sem_i: prog -> extra_val_t -> instr -> estate -> itree E estate)
-        (p : prog) (ev : extra_val_t).
-
-(* folding instruction semantics on commands *)
-Definition isem_foldr (c: cmd) : estate -> itree E estate :=
-  foldr (fun i k s => s' <- sem_i p ev i s ;; k s')
-        (fun s: estate => Ret s) c.
-
-(* Make global definition *)
-Local Notation continue_loop s := (ret (inl s)).
-Local Notation exit_loop s := (ret (inr s)).
-
-Definition isem_for_round (i : var_i) (c : cmd)
-  (w: Z) (k: estate -> itree E estate) (s: estate) :
-    itree E estate :=
-  s <- iwrite_var true i (Vint w) s ;;
-  s <- isem_foldr c s ;; k s.
-
-Definition isem_for_loop (i : var_i) (c : cmd) (ls : list Z)
-  : estate -> itree E estate :=
-  foldr (isem_for_round i c) (fun s: estate => Ret s) ls.
-
-Definition isem_while_round (c1 : cmd) (e : pexpr) (c2 : cmd) (s : estate) :
-    itree E (estate + estate) :=
-  s <- isem_foldr c1 s;;
-  b <- isem_cond p e s;;
-  if b then s <- isem_foldr c2 s;; continue_loop s
-  else exit_loop s.
-
-Definition isem_while_loop (c1 : cmd) (e:pexpr) (c2: cmd) (s : estate) :
-    itree E estate :=
-  ITree.iter (isem_while_round c1 e c2) s.
-
-End SEM_C.
-
-Class sem_Fun (E : Type -> Type) :=
-  { sem_fun : prog -> extra_val_t -> funname -> fstate -> itree E fstate }.
-
-#[global]
-Instance sem_fun_rec (E : Type -> Type) : sem_Fun (recCall +' E) | 0 :=
-  {| sem_fun := fun _ _ => rec_call (E:=E) |}.
-
-Section SEM_I.
-
-Context {E E0} {wE : with_Error E E0} {sem_F : sem_Fun E }.
-
-(* semantics of instructions, abstracting on function calls (through
-   sem_fun) *)
-Fixpoint isem_i_body (p : prog) (ev : extra_val_t) (i : instr) (s : estate) :
-    itree E estate :=
-  let: (MkI _ i) := i in
-  match i with
-  | Cassgn x tg ty e => iresult s (sem_assgn p x tg ty e s)
-
-  | Copn xs tg o es => iresult s (sem_sopn (p_globs p) o s xs es)
-
-  | Csyscall xs o es => iresult s (sem_syscall p xs o es s)
-
-  | Cif e c1 c2 =>
-    b <- isem_cond p e s;;
-    isem_foldr isem_i_body p ev (if b then c1 else c2) s
-
-  | Cwhile a c1 e i c2 =>
-    isem_while_loop isem_i_body p ev c1 e c2 s
-
-  | Cfor i (d, lo, hi) c =>
-    bounds <- isem_bound p lo hi s;;
-    isem_for_loop isem_i_body p ev i c (wrange d bounds.1 bounds.2) s
-
-  | Ccall xs fn args =>
-    vargs <- isem_pexprs  (~~direct_call) (p_globs p) args s;;
-    fs <- sem_fun p ev fn (mk_fstate vargs s) ;;
-    iresult s (upd_estate (~~direct_call) (p_globs p) xs fs s)
-  end.
-(* similar, for commands *)
-Definition isem_cmd_ := isem_foldr isem_i_body.
-
-Lemma isem_cmd_cat p ev c c' s :
-  isem_cmd_ p ev (c ++ c') s ≈ (s <- isem_cmd_ p ev c s;; isem_cmd_ p ev c' s).
-Proof.
-  rewrite /isem_cmd_; elim: c s => [ | i c hc] /= s.
-  + rewrite bind_ret_l; reflexivity.
-  rewrite bind_bind; setoid_rewrite hc; reflexivity.
-Qed.
-
-Lemma isem_cmd_while p ev ii al c e inf c' s:
-  isem_cmd_ p ev [:: MkI ii (Cwhile al c e inf c')] s
-  ≈
- isem_cmd_ p ev (c ++ [:: MkI ii (Cif e (c' ++ [:: MkI ii (Cwhile al c e inf c')]) [::])]) s.
-Proof.
-  rewrite /= isem_cmd_cat.
-  rewrite /isem_while_loop unfold_iter bind_ret_r.
-  rewrite /isem_while_round bind_bind /isem_cmd_.
-  apply eutt_eq_bind => {}s /=; rewrite !bind_bind.
-  apply eutt_eq_bind => -[] /=; last by rewrite !bind_ret_l; reflexivity.
-  rewrite -/isem_cmd_ isem_cmd_cat; rewrite !bind_bind.
-  apply eutt_eq_bind => {}s /= ; rewrite bind_ret_l !bind_ret_r tau_eutt; reflexivity.
-Qed.
-
-Definition estate0 (fs : fstate) :=
-  Estate fs.(fscs) fs.(fmem) Vm.init.
-
-Definition initialize_funcall (p : prog) (ev : extra_val_t) (fd : fundef) (fs : fstate) : exec estate :=
-  let sinit := estate0 fs in
-  Let vargs' := mapM2 ErrType dc_truncate_val fd.(f_tyin) fs.(fvals) in
-  Let s0 := init_state fd.(f_extra) (p_extra p) ev sinit in
-  write_vars (~~direct_call) fd.(f_params) vargs' s0.
-
-Definition finalize_funcall (fd : fundef) (s:estate) : exec fstate :=
-  Let vres := get_var_is (~~ direct_call) s.(evm) fd.(f_res) in
-  Let vres' := mapM2 ErrType dc_truncate_val fd.(f_tyout) vres in
-  let scs := s.(escs) in
-  let m := finalize fd.(f_extra) s.(emem) in
-  ok {| fscs := scs; fmem := m; fvals := vres' |}.
-
-Definition ifinalize_funcall (fd : fundef) (s:estate) : itree E fstate :=
-  err_result (fun e => (e, tt)) (finalize_funcall fd s).
-
-(* similar, for proper function calls *)
-Definition isem_fun_body (p : prog) (ev : extra_val_t)
-   (fn : funname) (fs : fstate) :=
-   fd <- kget_fundef (p_funcs p) fn fs;;
-   let sinit := estate0 fs in
-   s1 <- iresult sinit (initialize_funcall p ev fd fs);;
-   s2 <- isem_cmd_ p ev fd.(f_body) s1;;
-   iresult s2 (finalize_funcall fd s2).
-
-(* A variant of the semantic based on exec, usefull for the proofs *)
-Fixpoint esem_i (p : prog) (ev : extra_val_t) (i : instr) (s : estate) :
-    exec estate :=
-  let: (MkI ii i) := i in
-  match i with
-  | Cassgn x tg ty e => sem_assgn p x tg ty e s
-
-  | Copn xs tg o es => sem_sopn (p_globs p) o s xs es
-
-  | Csyscall xs o es => sem_syscall p xs o es s
-
-  | Cif e c1 c2 =>
-    Let b := sem_cond (p_globs p) e s in
-    foldM (esem_i p ev) s (if b then c1 else c2)
-
-  | Cwhile a c1 e i c2 => Error ErrSemUndef
-
-  | Cfor i (d, lo, hi) c =>
-    Let bounds := sem_bound (p_globs p) lo hi s in
-    foldM (fun j s =>
-      Let s := write_var true i (Vint j) s in
-      foldM (esem_i p ev) s c)
-     s (wrange d bounds.1 bounds.2)
-
-  | Ccall xs fn args => Error ErrSemUndef
-  end.
-
-Definition esem (p : prog) (ev : extra_val_t) (c : cmd) (s : estate) :=
-  foldM (esem_i p ev) s c.
-
-Definition esem_for p ev i c :=
-  foldM (fun j s =>
-      Let s := write_var true i (Vint j) s in
-      foldM (esem_i p ev) s c).
-
-Lemma esem_i_bodyP p ev c s s' :
-  esem p ev c s = ok s' -> isem_cmd_ p ev c s ≈ iresult s (ok s').
-Proof.
-  set Pi := fun i => forall s s', esem_i p ev i s = ok s' -> isem_i_body p ev i s ≈ iresult s (ok s').
-  set Pi_r := fun i => forall ii, Pi (MkI ii i).
-  set Pc := fun c => forall s s', foldM (esem_i p ev) s c = ok s' -> isem_cmd_ p ev c s ≈ iresult s (ok s').
-  apply (cmd_rect (Pr := Pi_r) (Pi := Pi) (Pc := Pc)) => {s s' c} //.
-  + move=> > /= [<-]; reflexivity.
-  + by move=> i c hi hc s s' /=; t_xrbindP => s1 /hi ->; rewrite bind_ret_l; apply hc.
-  1-3: move=> > /= -> /=; reflexivity.
-  + move=> > hc1 hc2 ii s s' /=.
-    rewrite /isem_cond; t_xrbindP => b -> /=.
-    by rewrite bind_ret_l; case: b; [apply hc1 | apply hc2].
-  move=> i d lo hi c hc ii s s' /=.
-  rewrite /isem_bound; t_xrbindP => bound -> /=.
-  rewrite bind_ret_l.
-  elim: wrange s => {bound} => /= [ | j js hrec] s.
-  + move=> [<-]; reflexivity.
-  t_xrbindP => s1 s2 hw /hc{}hc /hrec{}hrec.
-  rewrite /isem_for_round /= /iwrite_var hw /= bind_ret_l.
-  by move: hc; rewrite /isem_cmd_ => -> /=; rewrite bind_ret_l.
-Qed.
-
-Lemma esem_cat p ev c1 c2 s : esem p ev (c1 ++ c2) s = Let s1 := esem p ev c1 s in esem p ev c2 s1.
-Proof. by rewrite /esem foldM_cat. Qed.
-
-Lemma esem_cons p ev i c s : esem p ev (i :: c) s = Let s1 := esem_i p ev i s in esem p ev c s1.
-Proof. done. Qed.
-
-Lemma esem_c_nil p ev s : esem p ev [::] s = ok s.
-Proof. done. Qed.
-
-Lemma eEForOne p ev s1 s1' s2 s3 i w ws c :
-  write_var true i (Vint w) s1 = ok s1' ->
-  esem p ev c s1' = ok s2 ->
-  esem_for p ev i c s2 ws = ok s3 ->
-  esem_for p ev i c s1 (w :: ws) = ok s3.
-Proof. by rewrite /esem => /= -> /= -> /=. Qed.
-
-End SEM_I.
-
-(*** error-aware interpreter with recursion ***************************)
-Section SEM_F.
-
-Context {E E0} {wE : with_Error E E0}.
-
-(* semantics of instructions parametrized by recCall events *)
-Definition isem_i_rec (p : prog) (ev : extra_val_t) (i : instr) (s : estate)
-  : itree (recCall +' E) estate :=
-  isem_i_body p ev i s.
-
-(* similar, for commands *)
-Definition isem_cmd_rec (p : prog) (ev : extra_val_t) (c : cmd) (s : estate)
-  : itree (recCall +' E) estate :=
-  isem_cmd_ p ev c s.
-
-(* similar, for function calls *)
-Definition isem_fun_rec (p : prog) (ev : extra_val_t)
-   (fn : funname) (fs : fstate) : itree (recCall +' E) fstate :=
-  isem_fun_body p ev fn fs.
-
-(* handler of recCall events *)
-Definition handle_recCall (p : prog) (ev : extra_val_t) :
-   recCall ~> itree (recCall +' E) :=
- fun T (rc : recCall T) =>
-   match rc with
-   | RecCall fn fs => isem_fun_rec p ev fn fs
-   end.
-
-(* intepreter of recCall events for functions, giving us the recursive
-   semantics of functions *)
-Definition isem_fun (p : prog) (ev : extra_val_t) (fn : funname) (fs : fstate) : itree E fstate :=
-  mrec (handle_recCall p ev) (RecCall fn fs).
-
-#[global]
-Instance sem_fun_full : sem_Fun E | 100 :=
-  {| sem_fun := isem_fun |}.
-
-(* recursive semantics of instructions *)
-Definition isem_i (p : prog) (ev : extra_val_t) (i : instr) (s : estate) : itree E estate :=
-  isem_i_body p ev i s.
-
-(* similar, for commands *)
-Definition isem_cmd (p : prog) (ev : extra_val_t) (c : cmd) (s : estate) : itree E estate :=
-  isem_cmd_ p ev c s.
-
-End SEM_F.
-
-(* interpreter of error events, giving us the fully interpreted
-   semantics of functions *)
-Definition err_sem_fun (p : prog) (ev : extra_val_t) (fn : funname)
-    (fs : fstate) : execT (itree void1) fstate :=
-  interp_Err (isem_fun p ev fn fs).
-
-(*** Core lemmas about the definition ********************************)
-Section CoreLemmas.
-
-Context {E E0: Type -> Type} {wE : with_Error E E0}.
-Context (p : prog) (ev : extra_val_t).
-
-Notation interp_rec := (interp (mrecursive (handle_recCall p ev))).
-
-Lemma interp_throw T e : interp_rec (throw (X:=T) e) ≈ throw e.
-Proof. rewrite interp_vis bind_trigger; apply eqit_Vis => -[]. Qed.
-
-Lemma interp_err_result e T (r : result error T) :
-  eutt (E:=E) eq (interp_rec (err_result e r)) (err_result e r).
-Proof.
-  case: r => /= [t | err].
-  + rewrite interp_ret; reflexivity.
-  apply interp_throw.
-Qed.
-
-Lemma interp_ioget Err T (o : option T) :
-  eutt (E:=E) eq (interp_rec (ioget Err o)) (ioget Err o).
-Proof.
-  case o => /= [? | ].
-  + rewrite interp_ret; reflexivity.
-  apply interp_throw.
-Qed.
-
-Lemma interp_iresult s T (r : exec T) :
-  eutt (E:=E) eq (interp (mrecursive (handle_recCall p ev)) (iresult s r)) (iresult s r).
-Proof.
-  case r => /= [? | ?].
-  + rewrite interp_ret; reflexivity.
-  apply interp_throw.
- Qed.
-
-Lemma interp_isem_cmd c s :
-  eutt (E:=E) eq (interp_rec (isem_foldr isem_i_rec p ev c s))
-         (isem_foldr isem_i_body p ev c s).
-Proof.
-  apply:
-   (cmd_rect
-    (Pr := fun ir => forall ii s,
-       eutt (E:=E) eq (interp_rec (isem_i_rec p ev (MkI ii ir) s))
-                      (isem_i p ev (MkI ii ir) s))
-    (Pi := fun i => forall s,
-       eutt (E:=E) eq (interp_rec (isem_i_rec p ev i s))
-                      (isem_i p ev i s))
-    (Pc := fun c => forall s,
-       eutt (E:=E) eq (interp_rec (isem_foldr isem_i_rec p ev c s))
-                      (isem_cmd p ev c s))) => // {c s}.
-  + move=> s /=; rewrite interp_ret; reflexivity.
-  + move=> i c hi hc s; rewrite interp_bind;apply eqit_bind; first by apply hi.
-    by move=> s'; apply hc.
-  1-3: by move=> >; apply interp_iresult.
-  + move=> e c1 c2 hc1 hc2 ii s; rewrite /isem_i /isem_i_rec /=.
-    rewrite interp_bind; apply eqit_bind.
-    + by apply interp_iresult.
-    by move=> []; [apply hc1 | apply hc2].
-  + move=> v dir lo hi c hc ii s; rewrite /isem_i /isem_i_rec /=.
-    rewrite interp_bind; apply eqit_bind; first by apply interp_iresult.
-    move=> bounds /=. elim: wrange s => {bounds ii} //=.
-    + move=> >; rewrite interp_ret; reflexivity.
-    move=> j js hrec s.
-    rewrite interp_bind; apply eqit_bind; first by apply interp_iresult.
-    move=> s'; rewrite interp_bind.
-    rewrite hc; setoid_rewrite hrec; reflexivity.
-  + move=> al c1 e inf c2 hc1 hc2 ii s; rewrite /isem_i /isem_i_rec /= /isem_while_loop.
-    rewrite interp_iter; apply eutt_iter=> {}s.
-    rewrite /isem_while_round.
-    rewrite interp_bind; apply eqit_bind; first by apply hc1.
-    move=> s1; rewrite interp_bind; apply eqit_bind; first by apply interp_iresult.
-    move=> [].
-    + rewrite interp_bind; apply eqit_bind; first by apply hc2.
-      move=> s2; rewrite interp_ret; reflexivity.
-    rewrite interp_ret; reflexivity.
-  move=> xs f es ii s; rewrite /isem_i /isem_i_rec /=.
-  rewrite interp_bind; apply eqit_bind; first by apply interp_iresult.
-  move=> vs.
-  rewrite interp_bind; apply eqit_bind; last by move=> >; apply interp_iresult.
-  rewrite interp_mrecursive; reflexivity.
-Qed.
-
-Lemma isem_call_unfold (fn : funname) (fs : fstate) :
-  isem_fun p ev fn fs ≈ isem_fun_body p ev fn fs.
-Proof.
-  rewrite {1}/isem_fun.
-  rewrite mrec_as_interp.
-  rewrite {2}/handle_recCall /isem_fun_rec /isem_fun_body.
-  rewrite interp_bind; apply eqit_bind.
-  + by apply interp_ioget.
-  move=> fd; rewrite interp_bind; apply eqit_bind.
-  + by apply interp_iresult.
-  move=> s1; rewrite interp_bind; apply eqit_bind.
-  + apply interp_isem_cmd.
-  move=> s2; apply interp_iresult.
-Qed.
-
-End CoreLemmas.
-
-End WSW.
